refactor

Rlist.v
@@ -11,6 +11,9 @@ Unset Elimination Schemes.
 Inductive Rlist (R : Type) (A : Type) := rnode of (R -> Rnode R A)
 with Rnode (R : Type) (A : Type) := rnil | rcons of A & Rlist R A.
 
+Definition unwrap {R A} (l : Rlist R A) : R -> Rnode R A :=
+  let: rnode n := l in n.
+
 Lemma eq_rnode {R A}:
   forall f1 f2 : R -> Rnode R A,
   (forall r, f1 r = f2 r) ->
@@ -30,8 +33,7 @@ Definition cons {R A} (x : R -> A) (l : Rlist R A) : Rlist R A :=
 Definition lift {R A} (x : A) := @rnode R A (fun _ => rcons x nil).
 
 Fixpoint run {R A} (l : Rlist R A) (r : R) : seq A :=
-  let: rnode n := l in
-  run_node (n r) r
+  run_node (unwrap l r) r
 
 with run_node {R A} (n : Rnode R A) (r : R) : seq A :=
 match n with
@@ -40,12 +42,11 @@ match n with
 end.
 
 Fixpoint cat {R A} (l1 l2 : Rlist R A) : Rlist R A :=
-  let: rnode n := l1 in
-  rnode (fun r => cat_node (n r) l2 r)
+  rnode (fun r => cat_node (unwrap l1 r) l2 r)
 
 with cat_node {R A} (n : Rnode R A) (l2 : Rlist R A) : R -> Rnode R A :=
 match n with
-| rnil => let: rnode n := l2 in n
+| rnil => unwrap l2
 | rcons x l1 => fun _ => rcons x (cat l1 l2)
 end.
 
@@ -73,8 +74,7 @@ by move=>?????; rewrite cat_assoc.
 Qed.
 
 Fixpoint map {R A B} (f : A -> B) (l : Rlist R A) : Rlist R B :=
-  let: rnode n := l in
-  rnode (fun r => map_node f (n r))
+  rnode (map_node f \o unwrap l)
 with map_node {R A B} (f : A -> B) (n : Rnode R A) :=
 match n with
 | rnil => rnil
@@ -86,7 +86,7 @@ Lemma map_cat {R A B}: forall (f : A -> B) (l1 l2 : Rlist R A),
 with map_cat_node {R A B}: forall (f : A -> B) (n1 : Rnode R A) l2 r,
   map_node f (cat_node n1 l2 r) = cat_node (map_node f n1) (map f l2) r.
 Proof.
-- by move=>?[?]?/=; under eq_rnode=>? do rewrite map_cat_node.
+- by move=>?[?]?/=; under eq_rnode=>? do rewrite /= map_cat_node.
 move=>?; case=>/=; first by case.
 by move=>????; rewrite map_cat.
 Qed.
@@ -96,7 +96,7 @@ Lemma map_map {R A B C} : forall (f : A -> B) (g : B -> C) (l : Rlist R A),
 with map_map_node {R A B C} : forall (f : A -> B) (g : B -> C) (n : Rnode R A),
   map_node g (map_node f n) = map_node (g \o f) n.
 Proof.
-- by move=>??[?]/=; under eq_rnode=>? do rewrite map_map_node.
+- by move=>??[?]/=; under eq_rnode=>? do rewrite /= map_map_node.
 move=>??; case=>//=??.
 by rewrite map_map.
 Qed.
@@ -104,13 +104,12 @@ Qed.
 Lemma map_id {R A} : forall l : Rlist R A, map id l = l
 with map_id_node {R A} : forall n : Rnode R A, map_node id n = n.
 Proof.
-- by case=>?/=; under eq_rnode=>? do rewrite map_id_node.
+- by case=>?/=; under eq_rnode=>? do rewrite /= map_id_node.
 by case=>//=??; rewrite map_id.
 Qed.
 
 Fixpoint set {R S A} (g : S -> R) (l : Rlist R A) : Rlist S A :=
-  let: rnode n := l in
-  rnode (fun r => set_node g (n (g r)))
+  rnode (set_node g \o unwrap l \o g)
 with set_node {R S A} (g : S -> R) (n : Rnode R A) :=
 match n with
 | rnil => rnil
@@ -122,7 +121,7 @@ Lemma set_cat {R S A} : forall (g : S -> R) (l1 l2 : Rlist R A),
 with set_cat_node {R S A} : forall (g : S -> R) (n1 : Rnode R A) l2 r,
   set_node g (cat_node n1 l2 (g r)) = cat_node (set_node g n1) (set g l2) r.
 Proof.
-- by move=>?[?]?/=; under eq_rnode=>? do rewrite set_cat_node.
+- by move=>?[?]?/=; under eq_rnode=>? do rewrite /= set_cat_node.
 move=>?; case=>/=; first by case.
 by move=>????; rewrite set_cat.
 Qed.
@@ -132,7 +131,7 @@ Lemma map_set {R S A B} : forall (f : A -> B) (g : S -> R) l,
 with map_set_node {R S A B} : forall (f : A -> B) (g : S -> R) n,
   map_node f (set_node g n) = set_node g (map_node f n).
 Proof.
-- by move=>??[?]/=; under eq_rnode=>? do rewrite map_set_node.
+- by move=>??[?]/=; under eq_rnode=>? do rewrite /= map_set_node.
 move=>??; case=>//=??.
 by rewrite map_set.
 Qed.
@@ -142,7 +141,7 @@ Lemma set_set {R S T A} : forall (f : S -> R) (g : T -> S) (l : Rlist R A),
 with set_set_node {R S T A} : forall (f : S -> R) (g : T -> S) (n : Rnode R A),
   set_node g (set_node f n) = set_node (f \o g) n.
 Proof.
-- by move=>??[?]/=; under eq_rnode=>? do rewrite set_set_node.
+- by move=>??[?]/=; under eq_rnode=>? do rewrite /= set_set_node.
 move=>??; case=>//=??.
 by rewrite set_set.
 Qed.
@@ -150,18 +149,17 @@ Qed.
 Lemma set_id {R A} : forall l : Rlist R A, set id l = l
 with set_id_node {R A} : forall (n : Rnode R A), set_node id n = n.
 Proof.
-- by case=>?/=; under eq_rnode=>? do rewrite set_id_node.
+- by case=>?/=; under eq_rnode=>? do rewrite /= set_id_node.
 by case=>//=??; rewrite set_id.
 Qed.
 
 Fixpoint concat {R A} (l : Rlist R (Rlist R A)) : Rlist R A :=
-  let: rnode n := l in
-  rnode (fun r => concat_node (n r) r)
+  rnode (fun r => concat_node (unwrap l r) r)
 
 with concat_node {R A} (n : Rnode R (Rlist R A)) : R -> Rnode R A :=
 match n with
 | rnil => fun _ => rnil
-| rcons x l => fun r => let: rnode n := cat x (concat l) in n r
+| rcons x l => unwrap (cat x (concat l))
 end.
 
 Lemma concat_cat {R A} : forall l1 l2 : Rlist R (Rlist R A),
@@ -190,7 +188,7 @@ Lemma map_concat {R A B} : forall (f : A -> B) (l : Rlist R (Rlist R A)),
 with map_concat_node {R A B} : forall (f : A -> B) (n : Rnode R (Rlist R A)) r,
   map_node f (concat_node n r) = concat_node (map_node (map f) n) r.
 Proof.
-- by move=>?[?]/=; under eq_rnode=>? do rewrite map_concat_node.
+- by move=>?[?]/=; under eq_rnode=>? do rewrite /= map_concat_node.
 move=>?; case=>//=; case=>???/=.
 by rewrite map_cat_node map_concat.
 Qed.
@@ -200,7 +198,7 @@ Lemma set_concat {R S A} : forall (g : S -> R) (l : Rlist R (Rlist R A)),
 with set_concat_node {R S A} : forall (g : S -> R) (n : Rnode R (Rlist R A)) r,
   set_node g (concat_node n (g r)) = concat_node (set_node g (map_node (set g) n)) r.
 Proof.
-- by move=>?[?]/=; under eq_rnode=>? do rewrite set_concat_node.
+- by move=>?[?]/=; under eq_rnode=>? do rewrite /= set_concat_node.
 move=>?; case=>//=; case=>???/=.
 by rewrite set_cat_node set_concat.
 Qed.
@@ -215,7 +213,7 @@ by case: r.
 Qed.
 
 Definition collapse {R A} (f : R -> Rlist R A) : Rlist R A :=
-  rnode (fun r => let: rnode n := f r in n r).
+  rnode (fun r => unwrap (f r) r).
 
 Lemma collapse_cat {R A} : forall f g : R -> Rlist R A,
   collapse (fun r => cat (f r) (collapse g)) = cat (collapse f) (collapse g).
@@ -225,8 +223,7 @@ by apply: eq_rnode=>?; case: (f _).
 Qed.
 
 Fixpoint fold_right {R A B} (f : A -> (R -> B) -> (R -> B)) (accu : R -> B) (l : Rlist R A) (r : R) : B :=
-let: rnode n := l in
-fold_right_node f accu (n r) r
+fold_right_node f accu (unwrap l r) r
 
 with fold_right_node {R A B} (f : A -> (R -> B) -> (R -> B)) (accu : R -> B) (n : Rnode R A) (r : R) : B :=
 match n with
